RocqOfRust/revm/revm_interpreter/tests/host.v
@@ -68,6 +68,10 @@ Module TestHost.
       aliases.U256.t * t :=
     ({| Uint.value := 1 |}, Make).
 
+  Definition host_basefee (self : t) :
+      aliases.U256.t * t :=
+    (Impl_Uint.ZERO, Make).
+
   Definition balance (self : t) (_address : Address.t) :
       option (StateLoad.t aliases.U256.t) * t :=
     (None, Make).
@@ -233,6 +237,7 @@ Module TestHost.
     Host.block_hash := block_hash;
     Host.block_number := block_number;
     Host.chain_id := host_chain_id;
+    Host.basefee := host_basefee;
     Host.balance := balance;
     Host.code := code;
     Host.code_hash := code_hash;
@@ -309,6 +314,10 @@ Module TestHostWithAccount.
       aliases.U256.t * t :=
     ({| Uint.value := 1 |}, Make).
 
+  Definition host_basefee (self : t) :
+      aliases.U256.t * t :=
+    (Impl_Uint.ZERO, Make).
+
   Definition balance (self : t) (_address : Address.t) :
       option (StateLoad.t aliases.U256.t) * t :=
     (None, Make).
@@ -474,6 +483,7 @@ Module TestHostWithAccount.
     Host.block_hash := block_hash;
     Host.block_number := block_number;
     Host.chain_id := host_chain_id;
+    Host.basefee := host_basefee;
     Host.balance := balance;
     Host.code := code;
     Host.code_hash := code_hash;
